checking progress...

theories/L6_PCPS/Heap/closure_conversion_correct.v
@@ -23,44 +23,95 @@ Module ClosureConversionCorrect (H : Heap).
   
   Variable clo_tag : cTag.
   
-    
-  Definition FP k i (H : heap block) (rho1 : env) (e1 : exp)
+  (** * Postcondition *)
+  (** Enforces that the resource consumption of the target is within certain bounds *)
+  Definition Post
+             k (* time units already spent *)
+             i (* step index *)
+             (p1 p2 : heap block * env * exp * nat * nat) :=
+    match p1, p2 with
+      | (H1, rho1, e1, c1, m1), (H2, rho2, e2, c2, m2) =>
+        c1 <= c2 + k <= 7 * c1 * (max_exp_env i H1 rho1 e1) + 7 * sizeOf_exp e1 /\
+        m1 <= m2 <= 4 * m1 * (max_exp_env i H1 rho1 e1) + 4 * sizeOf_exp e1
+    end.
+
+  (** Enforces that the resource consumption of the target is within certain bounds *)
+  Definition PostL
+             k (* time units already spent *)
+             i H1 rho1 e1
              (p1 p2 : nat * nat) :=
     match p1, p2 with
       | (c1, m1), (c2, m2) =>
-        c1 <= c2 + k <= 7 * c1 * (max_exp_env i H rho1 e1) + 7 * sizeOf_exp e1 /\
-        m1 <= m2 <= 4 * m1 * (max_exp_env i H rho1 e1) + 4 * sizeOf_exp e1
+        c1 <= c2 + k <= 7 * c1 * (max_exp_env i H1 rho1 e1) + 7 * sizeOf_exp e1 /\
+        m1 <= m2 <= 4 * m1 * (max_exp_env i H1 rho1 e1) + 4 * sizeOf_exp e1
     end.
   
-  Definition IP i C (p1 p2 : heap block * env * exp) :=
+  (** * Precondition *)
+  (** Enforces that the initial heaps have related sizes *)
+  Definition Pre
+             C (* Context already processed *)
+             i (* step index *)
+             (p1 p2 : heap block * env * exp) :=
     let m := cost_alloc_ctx C in 
     match p1, p2 with
       | (H1, rho1, e1), (H2, rho2, e2) =>
         size_heap H1 + m  <= size_heap H2 <=
         4 * (size_heap H1 + m) * (max_exp_env i H1 rho1 e1) + 4 * sizeOf_exp e1
     end.
-  
-  Lemma FP_transfer i (H1 : heap block) (rho1 : env) (e1 : exp)
+
+  (** * Properties of the cost invariants *)
+
+  (** Transfer units from the accumulator to the cost of e2 *)
+  Lemma Post_transfer i (H1 H2 : heap block) (rho1 rho2 : env) (e1 e2 : exp)
         (k c1 c2 c m1 m2 : nat) : 
-    FP (k + c) i H1 rho1 e1  (c1, m1) (c2, m2) -> FP k i H1 rho1 e1 (c1, m1) (c2 + c, m2).
+    Post (k + c) i (H1, rho1, e1, c1, m1) (H2, rho2, e2, c2, m2) ->
+    Post k i (H1, rho1, e1, c1, m1) (H2, rho2, e2, c2 + c, m2).
   Proof.
     simpl. intros H. omega.
   Qed.
+
+
+  (** TODO move *)
+
+  Lemma ctx_to_heap_env_size_heap C rho1 rho2 H1 H2 c :
+    ctx_to_heap_env C H1 rho1 H2 rho2 c ->
+    size_heap H2 = size_heap H1 + cost_alloc_ctx C.
+  Proof.
+    intros Hctx; induction Hctx; eauto.
+    simpl. rewrite IHHctx.
+    unfold size_heap.
+    erewrite (HL.size_with_measure_alloc _ _ _ H H');
+      [| reflexivity | eassumption ].
+    erewrite getlist_length_eq; [| eassumption ].
+    simpl. omega.
+  Qed.
+
+  (** Process the evaluation context of the right expression *)
+  Lemma IP_ctx_to_heap_env
+        i (H1 H2 H2' : heap block) (rho1 rho2 rho2' : env)
+        (e1 e2 : exp) (C C' : exp_ctx) (c : nat) : 
+    Pre C' i (H1, rho1, e1) (H2, rho2, C |[ e2 ]|) ->
+    ctx_to_heap_env C H2 rho2 H2' rho2' c ->
+    Pre (comp_ctx_f C' C) i (H1, rho1, e1) (H2', rho2', e2).
+  Proof.
+    intros [HP1 Hp2] Hctx. unfold Pre in *.
+    erewrite (ctx_to_heap_env_size_heap C rho2 rho2' H2 H2'); [| eassumption ].
+    rewrite cost_alloc_ctx_comp_ctx_f in *. split. omega.
+    assert (Hgrt1 := max_exp_env_grt_1 i H1 rho1 e1).
+    eapply le_trans. eapply plus_le_compat_r. eassumption.
+    rewrite plus_assoc.
+    rewrite <- (mult_assoc _ (size_heap H1 + cost_alloc_ctx C' + cost_alloc_ctx C)).
+    rewrite Nat.mul_add_distr_r. rewrite Nat.mul_add_distr_l.
+    rewrite Nat.mul_add_distr_l.  rewrite <- !plus_assoc. eapply plus_le_compat.
+    rewrite <- Nat.mul_add_distr_l. rewrite <- mult_assoc. omega.
+    rewrite plus_comm. eapply plus_le_compat_r.
+    eapply le_trans;
+      [| eapply mult_le_compat_l; eapply mult_le_compat_l; eassumption ].
+    omega. 
+  Qed.
   
-  (* Lemma ctx_to_heap_env_size_heap C rho1 rho2 H1 H2 c : *)
-  (*   ctx_to_heap_env C H1 rho1 H2 rho2 c -> *)
-  (*   size_heap H2 = size_heap H1 + cost_alloc_ctx C.  *)
-  (* Proof. *)
-  (*   intros Hctx; induction Hctx; eauto. *)
-  (*   simpl. rewrite IHHctx. *)
-  (*   unfold size_heap. *)
-  (*   erewrite (HL.size_with_measure_alloc _ _ _ H H'); *)
-  (*     [| reflexivity | eassumption ]. *)
-  (*   erewrite getlist_length_eq; [| eassumption ].  *)
-  (*   simpl. omega. *)
-  (* Qed. *)
 
-
+  (** * Lemmas about [project_var] and [project_vars] *)
   
   Lemma project_var_get Scope Funs σ c Γ FVs S1 x x' C1 S2 rho1 H1 rho2 H2 m y:
     project_var clo_tag Scope Funs σ c Γ FVs S1 x x' C1 S2 ->
@@ -197,29 +248,116 @@ Module ClosureConversionCorrect (H : Heap).
       + exists H2'', rho2'', (s + s'). eapply ctx_to_heap_env_comp_ctx_f_r; eassumption.
   Qed.
 
-  Lemma IP_ctx_to_heap_env
-        i (H1 H2 H2' : heap block) (rho1 rho2 rho2' : env)
-        (e1 e2 : exp) (C C' : exp_ctx) (c : nat) : 
-    IP i C' (H1, rho1, e1) (H2, rho2, C |[ e2 ]|) ->
-    ctx_to_heap_env C H2 rho2 H2' rho2' c ->
-    IP i (comp_ctx_f C' C) (H1, rho1, e1) (H2', rho2', e2).
-  Proof.
-    intros [HP1 Hp2] Hctx. unfold IP in *.
-    erewrite (ctx_to_heap_env_size_heap C rho2 rho2' H2 H2'); [| eassumption ].
-    rewrite cost_alloc_ctx_comp_ctx_f in *. split. omega.
-    assert (Hgrt1 := max_exp_env_grt_1 i H1 rho1 e1).
-    eapply le_trans. eapply plus_le_compat_r. eassumption.
-    rewrite plus_assoc.
-    rewrite <- (mult_assoc _ (size_heap H1 + cost_alloc_ctx C' + cost_alloc_ctx C)).
-    rewrite Nat.mul_add_distr_r. rewrite Nat.mul_add_distr_l.
-    rewrite Nat.mul_add_distr_l.  rewrite <- !plus_assoc. eapply plus_le_compat.
-    rewrite <- Nat.mul_add_distr_l. rewrite <- mult_assoc. omega.
-    rewrite plus_comm. eapply plus_le_compat_r.
-    eapply le_trans;
-      [| eapply mult_le_compat_l; eapply mult_le_compat_l; eassumption ].
-    omega. 
+  (** [project_var] preserves env_locs in dom *)
+  Lemma project_var_env_locs Scope Funs σ c Γ FVs x x' C S S' e k rho H rho' H':
+    project_var clo_tag Scope Funs σ c Γ FVs S x x' C S' ->
+    ctx_to_heap_env C H rho H' rho' k ->
+    well_formed (reach' H (env_locs rho (occurs_free (C |[ e ]|)))) H ->
+    env_locs rho (occurs_free (C |[ e ]|)) \subset dom H ->
+    env_locs rho' (occurs_free e) \subset dom  H'.
+  Proof with (now eauto with Ensembles_DB). 
+    intros Hvar Hctx Hlocs Hwf. inv Hvar; inv Hctx.
+    - simpl; eauto.
+    - inv H15.
+      rewrite HL.alloc_dom; [| eassumption ].
+      eapply Included_trans. eapply env_locs_set_Inlcuded'.
+      eapply Included_Union_compat. reflexivity.
+      eapply Included_trans; [| eassumption ]. simpl. normalize_occurs_free...
+    - inv H18.
+      eapply Included_trans. eapply env_locs_set_Inlcuded'.
+      simpl. eapply Union_Included.
+      + eapply Included_trans; [| eapply reachable_in_dom; eauto ].
+        simpl. normalize_occurs_free.
+        rewrite (reach_unfold H' (env_locs rho (Γ |: (occurs_free e \\ [set x'])))).
+        eapply Included_Union_preserv_r. 
+        eapply Included_trans; [| eapply reach'_extensive ]. rewrite !env_locs_Union, env_locs_Singleton; eauto.
+        rewrite post_Union. eapply Included_Union_preserv_l. simpl.
+        rewrite post_Singleton; eauto.
+        simpl. eapply In_Union_list. eapply in_map.
+        eapply nthN_In. eassumption.
+      + eapply Included_trans; [| eassumption ]. simpl. normalize_occurs_free...
   Qed.
 
+  (** [project_var] preserves well-formedness *)
+  Lemma project_var_well_formed Scope Funs σ c Γ FVs x x' C S S' e k rho H rho' H':
+    project_var clo_tag Scope Funs σ c Γ FVs S x x' C S' ->
+    ctx_to_heap_env C H rho H' rho' k ->
+    (env_locs rho (occurs_free (C |[ e ]|))) \subset dom H ->
+    well_formed (reach' H (env_locs rho (occurs_free (C |[ e ]|)))) H ->
+    well_formed (reach' H' (env_locs rho' (occurs_free e))) H'.
+  Proof with (now eauto with Ensembles_DB). 
+    intros Hvar Hctx Hlocs Hwf. inv Hvar; inv Hctx.
+    - simpl; eauto.
+    - inv H15.
+      eapply well_formed_antimon; [| eapply well_formed_reach_alloc; try eassumption ].
+      + eapply reach'_set_monotonic. eapply env_locs_monotonic.
+        simpl. normalize_occurs_free.
+        rewrite <- Union_assoc.
+        eapply Included_Union_preserv_r. eapply Included_Union_Setminus.
+        now eauto with typeclass_instances.
+      + simpl. normalize_occurs_free. rewrite env_locs_Union, reach'_Union; eauto.
+        eapply Included_Union_preserv_l.
+        rewrite !FromList_cons, !FromList_nil, !env_locs_Union, env_locs_Empty_set, Union_Empty_set_neut_r.
+        simpl in *. destruct (M.get (σ x) rho) eqn:Hget; try congruence.
+        destruct (M.get Γ rho) eqn:Hget'; try congruence. inv H13.
+        simpl. rewrite Union_Empty_set_neut_r. rewrite !env_locs_Singleton; try eassumption.
+        eapply reach'_extensive.
+    - inv H18.
+      eapply well_formed_antimon; [| eapply well_formed_reach_set; try eassumption ].
+      + eapply reach'_set_monotonic. eapply env_locs_monotonic.
+        simpl. normalize_occurs_free.
+        rewrite <- Union_assoc.
+        eapply Included_Union_preserv_r. eapply Included_Union_Setminus.
+        now eauto with typeclass_instances.
+      + simpl. eapply well_formed_antimon; try eassumption.
+        simpl. normalize_occurs_free. rewrite (reach_unfold H' (env_locs rho (Γ |: (occurs_free e \\ [set x'])))).
+        eapply Included_Union_preserv_r. 
+        eapply reach'_set_monotonic. rewrite !env_locs_Union, env_locs_Singleton; eauto.
+        rewrite post_Union. eapply Included_Union_preserv_l. simpl.
+        rewrite post_Singleton; eauto.
+        simpl. eapply In_Union_list. eapply in_map.
+        eapply nthN_In. eassumption.
+  Qed.
+
+  Lemma project_vars_env_locs Scope Funs σ c Γ FVs xs xs' C S S' e k rho H rho' H':
+    project_vars clo_tag Scope Funs σ c Γ FVs S xs xs' C S' ->
+    ctx_to_heap_env C H rho H' rho' k ->
+    well_formed (reach' H (env_locs rho (occurs_free (C |[ e ]|)))) H ->
+    env_locs rho (occurs_free (C |[ e ]|)) \subset dom H ->
+    env_locs rho' (occurs_free e) \subset dom  H'.
+  Proof with (now eauto with Ensembles_DB). 
+    intros Hvar. revert rho H rho' H' k e. 
+    induction Hvar; intros rho1 H1 rho2 H2 k e Hctx Hlocs Hwf.
+    - inv Hctx. simpl in *; eauto.
+    - edestruct ctx_to_heap_env_comp_ctx_f_l as [rho3 [H3 [m1 [m2 [Hctx2 [Hctx3 Heq]]]]]].
+      eassumption. subst.
+      rewrite <- app_ctx_f_fuse in *.
+      eapply IHHvar; try eassumption.
+      eapply project_var_well_formed; try eassumption.
+      eapply project_var_env_locs; try eassumption. 
+  Qed.
+  
+  
+  Lemma project_vars_well_formed Scope Funs σ c Γ FVs xs xs' C S S' e k rho H rho' H':
+    project_vars clo_tag Scope Funs σ c Γ FVs S xs xs' C S' ->
+    ctx_to_heap_env C H rho H' rho' k ->
+    (env_locs rho (occurs_free (C |[ e ]|))) \subset dom H ->
+    well_formed (reach' H (env_locs rho (occurs_free (C |[ e ]|)))) H ->
+    well_formed (reach' H' (env_locs rho' (occurs_free e))) H'.
+  Proof with (now eauto with Ensembles_DB). 
+    intros Hvar. revert rho H rho' H' k e. 
+    induction Hvar; intros rho1 H1 rho2 H2 k e Hctx Hlocs Hwf.
+    - inv Hctx. simpl in *; eauto.
+    - edestruct ctx_to_heap_env_comp_ctx_f_l as [rho3 [H3 [m1 [m2 [Hctx2 [Hctx3 Heq]]]]]].
+      eassumption. subst.
+      rewrite <- app_ctx_f_fuse in *.
+      eapply IHHvar; try eassumption.
+      eapply project_var_env_locs; try eassumption.
+      eapply project_var_well_formed; try eassumption. 
+  Qed.
+  
+      
+  (** * Lemmas about [Fun_inv] *)
   Lemma Fun_inv_weak_in_Fun_inv k P1 P2 rho1 H1 rho2 H2 β Scope Funs σ c Γ :
     Fun_inv k P1 P2 β rho1 H1 rho2 H2 Scope Funs σ c Γ ->
     Fun_inv_weak rho1 rho2 Scope Funs σ c Γ.
@@ -228,7 +366,8 @@ Module ClosureConversionCorrect (H : Heap).
     edestruct HFun as
         [vf [venv [Hnin' [Hget1 [Hget2 _]]]]]; eauto.
   Qed.
-  
+
+  (** * Lemmas about [FV_inv] *)
   Lemma FV_inv_weak_in_FV_inv k P1 P2 rho1 H1 rho2 H2 β Scope Funs c Γ FVs :
     FV_inv k P1 P2 β rho1 H1 rho2 H2 Scope Funs c Γ FVs ->
     FV_inv_weak rho1 rho2 H2 Scope Funs c Γ FVs.
@@ -244,14 +383,13 @@ Module ClosureConversionCorrect (H : Heap).
         (Scope Funs : Ensemble var) (FVs : list var)
         (σ : var -> var) (β : Inj) (c : cTag) (Γ : var) :
     (* [Scope] invariant *)
-    (forall j, (H1, rho1) ⋞ ^ (Scope ; k ; j ; IP k Hole_c ; FP 0 k H1 rho1 e1 ; β) (H2, rho2)) ->
+    (forall j, (H1, rho1) ⋞ ^ (Scope ; k ; j ; Pre Hole_c ; Post 0 ; β) (H2, rho2)) ->
     (* [Fun] invariant *)
-    Fun_inv k (IP k Hole_c) (FP 0 k H1 rho1 e1) β rho1 H1 rho2 H2 Scope Funs σ c Γ ->
+    Fun_inv k (Pre Hole_c) (Post 0) β rho1 H1 rho2 H2 Scope Funs σ c Γ ->
     (* Free variables invariant *)
-    FV_inv k (IP k Hole_c) (FP 0 k H1 rho1 e1) β rho1 H1 rho2 H2 Scope Funs c Γ FVs ->
+    FV_inv k (Pre Hole_c) (Post 0) β rho1 H1 rho2 H2 Scope Funs c Γ FVs ->
     (* location renaming is injective *)
     injective_subdomain (reach H1 (env_locs rho1 Scope)) β ->
-
     
     (* well-formedness *)
     well_formed (reach' H1 (env_locs rho1 (occurs_free e1))) H1 ->
@@ -274,7 +412,7 @@ Module ClosureConversionCorrect (H : Heap).
     (* [e'] is the closure conversion of [e] *)
     Closure_conversion clo_tag Scope Funs σ c Γ FVs e1 e2 C ->
     
-    (forall j, (e1, rho1, H1) ⪯ ^ (k ; j ; IP k Hole_c ; IP k Hole_c; FP 0 k H1 rho1 e1 ; FP 0 k H1 rho1 e1) (C |[ e2 ]|, rho2, H2)).
+    (forall j, (e1, rho1, H1) ⪯ ^ (k ; j ; Pre Hole_c k ; Pre Hole_c; PostL 0 k H1 rho1 e1 ; Post 0) (C |[ e2 ]|, rho2, H2)).
   Proof with now eauto with Ensembles_DB.
     revert H1 H2 rho1 rho2 e1 e2 C Scope Funs FVs σ β c Γ.
     induction k as [k IHk] using lt_wf_rec1.
@@ -291,25 +429,70 @@ Module ClosureConversionCorrect (H : Heap).
       eapply Fun_inv_weak_in_Fun_inv; eassumption.
       eapply FV_inv_weak_in_FV_inv; eassumption.
 
-      intros j. 
+      intros j.
+      (* process right ctx *)
       eapply cc_approx_exp_right_ctx_compat
-        with (ILi := fun c => FP c  k H1 rho1 (Econstr v t l e1));
-        [ now intros; eapply FP_transfer; eauto | now intros; eapply IP_ctx_to_heap_env; eauto
+      with (ILi := fun c => PostL c k H1 rho1 (Econstr v t l e1)) (II := fun C => Pre C k);
+        [ now intros; eapply Post_transfer; eauto | now intros; eapply IP_ctx_to_heap_env; eauto
           | eassumption | eassumption | eassumption | eassumption | eassumption | ].
       rewrite <- plus_n_O.
+      replace (comp_ctx_f Hole_c C) with C by eauto.
+      (* process Econstr one the right and left *)
       eapply cc_approx_exp_constr_compat
-      with (ILi := fun c => FP c  k H1 rho1 (Econstr v t l e1));
+      with (ILi := fun c => PostL c k H1 rho1 (Econstr v t l e1))
+           (r2 := 0)
+           (IIL2 := Pre Hole_c (k - cost H1 rho1 (Econstr v t l e1)));
         [ | | | eassumption | | eassumption  | | | | ].
-      + admit. (* bounds *)
-      + admit. (* bounds *)
-      + admit. (* bounds *)
-      + admit. (* well_formed *)
-      + admit. (* env_locs *)
+      + admit. (* bounds timeout compat *)
+      + admit. (* bounds - pick F *)
+      + admit. (* pre - allocation *) (* TODO maybe we need less assumptions *)
+      + admit. (* well-formed project vars *)
+      + admit. (* env_locs project vars *)
       + admit. (* project_vars_correct *)
-      + admit. (* bounds *)
+      + admit. (* bounds -- find F *)
       + (* Inductive case *)
-        intros i vs1 vs2 l1 l2 H1' H2'' Hlt Ha1 Ha2 Hall. (* bounds *)
-       
+        intros vs1 vs2 l1 l2 H1' H2'' Hleq Ha1 Ha2 Hr1 Hr2 Hall.
+        (* monotonicity of the local invariant *)
+        eapply cc_approx_exp_rel_mon with (LP1 := PostL 0 (k - cost H1 rho1 (Econstr v t l e1)) H1' (M.set v (Loc l1) rho1) e1). 
+        (* Induction hypothesis *)
+        { eapply IHk;
+          [ | | | | | | | | | | | | eassumption | | eassumption ].
+          * simpl in *. omega.
+          * admit. (* cc env set alloc *)
+          * admit. (* fun inv env_set_alloc *)
+          * admit. (* FV inv env set alloc *)
+          * admit. (* inj subdomain extend *)
+          * eapply well_formed_antimon;
+            [| rewrite occurs_free_Econstr in Hwf1;
+               eapply well_formed_reach_alloc'; try eassumption ]. 
+            eapply reach'_set_monotonic. eapply env_locs_monotonic...
+            eapply Included_trans; [| eassumption ]. normalize_occurs_free...
+            rewrite env_locs_Union. eapply Included_trans. eassumption.
+            normalize_occurs_free. rewrite env_locs_Union...
+          * eapply Included_trans. now eapply env_locs_set_Inlcuded'.
+            rewrite HL.alloc_dom; [| eassumption ].
+            eapply Included_Union_compat. reflexivity.
+            eapply Included_trans; [| eassumption ].
+            normalize_occurs_free...
+          * admit. (* need to prove WF for project vars first *)
+          * eapply Included_trans. now eapply env_locs_set_Inlcuded'.
+            rewrite HL.alloc_dom; [| eassumption ].
+            eapply Included_Union_compat. reflexivity.
+            (* need to prove env_locs for project vars first *)
+            admit.
+          * now eauto.
+          * eapply binding_in_map_antimon; [| eapply binding_in_map_set; eassumption ].
+            eapply occurs_free_Econstr_Included.
+          * intros f Hfin. eauto.
+          * eapply Disjoint_Included_r;
+              [| eapply Disjoint_Included_l; [ apply image_monotonic | now apply Hd ]].
+            normalize_bound_var... now eauto with Ensembles_DB. }
+        { admit. }
+        
+    - (* case Eproj *)
+      inv Hcc.
+      admit.
+      
     - (* case Ecase nil *)
       inv Hcc.
       admit.
